fix chacha20poly1305

code/chacha20poly1305/Hacl.Chacha20Poly1305.fst
@@ -11,7 +11,7 @@ open Lib.ByteBuffer
 open Hacl.Impl.Chacha20Poly1305.Poly
 
 
-module Seq = Lib.Sequence
+module LSeq = Lib.Sequence
 module ST = FStar.HyperStack.ST
 module Spec = Spec.Chacha20Poly1305
 module Chacha = Hacl.Impl.Chacha20
@@ -20,16 +20,8 @@ module Chacha = Hacl.Impl.Chacha20
 #set-options "--z3rlimit 50 --max_fuel 0 --max_ifuel 0"
 
 let aead_encrypt k n aadlen aad mlen m cipher mac =
-  let h0 = ST.get() in
   Chacha.chacha20_encrypt mlen cipher m k n 1ul;
-  let h1 = ST.get() in
-  poly1305_do k n aadlen aad mlen cipher mac;
-  let h2 = ST.get() in
-  assert (
-    let poly_k = Seq.sub (Spec.Chacha20.chacha20_key_block0 (as_seq h0 k) (as_seq h0 n)) 0 32 in
-    Seq.equal (as_seq h2 mac)
-      (Spec.poly1305_do poly_k (v mlen) (as_seq h1 cipher) (v aadlen) (as_seq h1 aad))
-    )
+  poly1305_do k n aadlen aad mlen cipher mac
 
 let aead_decrypt k n aadlen aad mlen m cipher mac =
   push_frame();
@@ -39,11 +31,6 @@ let aead_decrypt k n aadlen aad mlen m cipher mac =
   // Compute the expected mac using Poly1305
   poly1305_do k n aadlen aad mlen cipher computed_mac;
   let h1 = get() in
-  assert (
-    let poly_k = Seq.sub (Spec.Chacha20.chacha20_key_block0 (as_seq h0 k) (as_seq h0 n)) 0 32 in
-    Seq.equal (as_seq h1 computed_mac)
-      (Spec.poly1305_do poly_k (v mlen) (as_seq h0 cipher) (v aadlen) (as_seq h0 aad))
-    );
   let res =
     if lbytes_eq computed_mac mac then (
       assert (Lib.ByteSequence.lbytes_eq (as_seq h1 computed_mac) (as_seq h1 mac));
